EvalCBV.v
@@ -9,36 +9,15 @@ Import ListNotations.
 Local Open Scope list_scope.
 Local Open Scope prog_scope.
 
-Inductive IsOpaque : expr -> Prop :=
-  | OPvar x : IsOpaque (Evar x)
-  | OPconstr c : IsOpaque (Econstr c)
-.
-
-Inductive general_arg :=
-  | Aapp (_ : expr)
-  | Atapp (_ : type)
-  | Afold (_ : type)
-  | Ahide 
-.
-
-Definition general_apply (f : expr) (a : general_arg) :=
-  match a with
-    | Aapp e => Eapp f e
-    | Atapp t => Etapp f t
-    | Afold t => Efold t f
-    | Ahide => Ehide f
-  end.
-
-Definition general_apply_many f args := fold_left general_apply args f.
-
-Definition app_many f args := fold_left Eapp args f.
-
 Inductive IsValue : expr -> Prop :=
+| Vvar x : IsValue (Evar x)
 | Vabs t e : IsValue (Eabs t e)
-| Vapp f args : 
-    IsOpaque f ->
-    (forall a, In (Aapp a) args -> IsValue a) ->
-    IsValue (general_apply_many f args)
+| Vtabs e : IsValue (Etabs e)
+| Vfold t v : IsValue v -> IsValue (Efold t v)
+| Vtt : IsValue Ett
+| Vpair a b : IsValue a -> IsValue b -> IsValue (Epair a b)
+| Vinl t v : IsValue v -> IsValue (Einl t v)
+| Vinr t v : IsValue v -> IsValue (Einr t v)
 .
 
 (* evaluation context *)
@@ -47,14 +26,17 @@ Inductive econtext :=
   | ECapp1 (f : econtext) (arg : expr)
   | ECapp2 (f : expr) (arg : econtext) : IsValue f -> econtext
   | EClet (t : type) (def : econtext) (main : expr)
-  | ECletrec (defs : list letrec_entry) (main : econtext) (* Only evaluate main. All the definitions are already values, since that are all functions *)
-  | ECmatch_pair (target : econtext) (_ : expr)
-  | ECmatch_sum (target : econtext) (a b : expr)
   | ECtapp (f : econtext) (t : type)
   | ECfold (t : type) (_ : econtext)
-  | ECunfold (t : type) (_ : econtext)
+  | ECunfold (_ : econtext)
   | EChide (_ : econtext)
   | ECunhide (_ : econtext)
+  | ECpair1 (a : econtext) (b : expr)
+  | ECpair2 (a : expr) (b : econtext) : IsValue a -> econtext
+  | ECinl (_ : type) (_ : econtext)
+  | ECinr (_ : type) (_ : econtext)
+  | ECmatch_pair (target : econtext) (_ : expr)
+  | ECmatch_sum (target : econtext) (a b : expr)
 .
 
 Fixpoint plug (c : econtext) (e : expr) : expr :=
@@ -63,24 +45,23 @@ Fixpoint plug (c : econtext) (e : expr) : expr :=
     | ECapp1 f arg => Eapp (plug f e) arg
     | ECapp2 f arg _ => Eapp f (plug arg e)
     | EClet t def main => Elet t (plug def e) main
-    | ECletrec defs main => Eletrec defs (plug main e)
-    | ECmatch_pair target k => Ematch_pair (plug target e) k
-    | ECmatch_sum target a b => Ematch_sum (plug target e) a b
     | ECtapp f t => Etapp (plug f e) t
     | ECfold t c => Efold t (plug c e)
-    | ECunfold t c => Eunfold t (plug c e)
+    | ECunfold c => Eunfold (plug c e)
     | EChide c => Ehide (plug c e)
     | ECunhide c => Eunhide (plug c e)
+    | ECpair1 a b => Epair (plug a e) b
+    | ECpair2 a b _ => Epair a (plug b e)
+    | ECinl t c => Einl t (plug c e)
+    | ECinr t c => Einr t (plug c e)
+    | ECmatch_pair target k => Ematch_pair (plug target e) k
+    | ECmatch_sum target a b => Ematch_sum (plug target e) a b
   end.
 
 Inductive step : expr -> expr -> Prop :=
   | STecontext c e1 e2 : step e1 e2 -> step (plug c e1) (plug c e2)
   | STapp t body arg : IsValue arg -> step (Eapp (Eabs t body) arg) (subst arg body)
   | STlet t v main : IsValue v -> step (Elet t v main) (subst v main)
-  | STletrec_instantiate defs c (n : nat) t e : 
-      find n defs = Some (t, e) -> 
-      step (Eletrec defs (plug c (Evar #n))) (Eletrec defs (plug c e))  (* the definitions are only simplified, but not making any recursive or mutual-recursive call. All these calls are made only in the evaluation of 'main' *)
-  | STletrec_finish defs v : IsValue v -> step (Eletrec defs v) v (* this is wrong *)
   (* missing some rules for letrec *)
   | STmatch_pair ta tb a b k : 
       IsValue a ->
@@ -93,9 +74,9 @@ Inductive step : expr -> expr -> Prop :=
       IsValue v ->
       step (Ematch_sum (Einr $$ ta $$ tb $$ v) k1 k2) (subst v k2)
   | STtapp body t : step (Etapp (Etabs body) t) (subst t body)
-  | STunfold_fold v t1 t2 : 
+  | STunfold_fold v t1 : 
       IsValue v ->
-      step (Eunfold t2 (Efold t1 v)) v
+      step (Eunfold (Efold t1 v)) v
   | STunhide_hide v :
       IsValue v ->
       step (Eunhide (Ehide v)) v
