Syntax.v
@@ -3,17 +3,8 @@ Require Import Complexity.
 
 Export Complexity.
 
-Inductive tconstr :=
-| TCunit
-| TCprod
-| TCsum
-(* | TCint *)
-.
-
 Inductive type :=
 | Tarrow (t1 : type) (time_cost : cexpr) (result_size : size) (t2 : type)
-(* basic types *)
-| Tconstr (_ : tconstr)
 (* polymorphism *)           
 | Tvar (x : var)
 | Tuniversal (time_cost : cexpr) (result_size : size) (t : type)
@@ -24,58 +15,36 @@ Inductive type :=
 | Trecur (t : type)
 (* to deal with statistics s2 and s3 *)
 | Thide (_ : type)
+(* basic types *)
+| Tunit
+| Tprod (_ _ : type)
+| Tsum (_ _ : type)
 .
 
 Coercion Tvar : var >-> type.
 
-Inductive constr :=
-| Ctt
-| Cpair
-| Cinl
-| Cinr
-.
-
 Inductive expr :=
   | Evar (x : var)
-  | Econstr (c : constr)
   | Eapp (f : expr) (arg : expr)
   | Eabs (t : type) (body : expr)
   | Elet (t : type) (def : expr) (main : expr)
-  (* 'Definition' means the RHS of := in letrec.
-     Each definition must be a function, so there is an implicit quantifier on the RHS of :=. The LHS of := are also implicitly quantified. For example:
-     letrec x := \a. a * x (a - 1) with
-            y := \b. b * y (b - 1) in
-            x 10 + y 20
-     is written as 
-     letrec #0 * #2 (#0 - 1) with   (#2, #1, #0 -> x, y, a)
-            #0 * #1 (#0 - 1) in     (#2, #1, #0 -> x, y, b)
-            #1 10 + #0 10           (#1, #0 -> x, y)  
-     This must-be-function restriction is necessary for the type system to work 
-   *)
-  | Eletrec (defs : list (type * type * expr)) (main : expr)
-  (* The handler can access #1 and #0 representing the components of the pair
-   *)              
+  | Etapp (e : expr) (t : type)
+  | Etabs (body : expr)
+  | Efold (_ : type) (_ : expr)
+  | Eunfold (_ : expr)
+  | Ehide (_ : expr)
+  | Eunhide (_ : expr)
+  | Ett
+  | Epair (_ _ : expr)
+  | Einl (_ : type) (_ : expr)
+  | Einr (_ : type) (_ : expr)
   | Ematch_pair (target : expr) (handler : expr)
   (* left and right can access #0 representing the corresponding payload *)
   | Ematch_sum (target : expr) (left right : expr)
   (* | Eabs_notype (e : expr) (* a version of Eabs used in match handlers, where type annotation is not needed *) *)
-  | Etapp (e : expr) (t : type)
-  | Etabs (body : expr)
-  | Efold (_ : type) (_ : expr)
-  | Eunfold (_ : type) (_ : expr)
-  | Ehide (_ : expr)
-  | Eunhide (_ : expr)
 .
 
-Definition letrec_entry := (type * type * expr)%type.
-
 Coercion Evar : var >-> expr.
-Coercion Econstr : constr >-> expr.
-
-Definition Epair := Econstr Cpair.
-Definition Einl := Econstr Cinl.
-Definition Einr := Econstr Cinr.
-Definition Ett := Econstr Ctt.
 
 Instance Apply_type_type_type : Apply type type type :=
   {
